refl

CTree/Refinement.lean
@@ -5,7 +5,7 @@ namespace CTree
   inductive RefineF {ε : Type → Type} {ρ σ : Type}
     (r : Rel ρ σ) (sim : PartENat → PartENat → CTree ε ρ → CTree ε σ → Prop)
     : PartENat → PartENat → CTree ε ρ → CTree ε σ → Prop
-  | coind {p1' p2' p1 p2 t1 t2}
+  | coind {p1 p2 t1 t2} (p1' p2' : PartENat)
       (h1 : p1' < p1) (h2 : p2' < p2) (h : sim p1' p2' t1 t2)
       : RefineF r sim p1 p2 t1 t2
   | ret {x y p1 p2} (h : r x y) : RefineF r sim p1 p2 (ret x) (ret y)
@@ -29,7 +29,7 @@ namespace CTree
     greatest_fixpoint monotonicity by
       intro _ _ hsim _ _ _ _ h
       induction h with
-      | coind h1 h2 h => exact .coind h1 h2 (hsim _ _ _ _ h)
+      | coind _ _ h1 h2 h => exact .coind _ _ h1 h2 (hsim _ _ _ _ h)
       | ret h => exact .ret h
       | vis _ ih => exact .vis λ a => ih a
       | tau_left _ ih => exact RefineF.tau_left ih
@@ -46,12 +46,50 @@ namespace CTree
   notation:60 t1:61 " ⊑"r:61"⊑ " t2:61 => Refine r t1 t2
 
   theorem Refine.coind (sim : PartENat → PartENat → CTree ε ρ → CTree ε σ → Prop) (adm : ∀ p1 p2 t1 t2, sim p1 p2 t1 t2 → RefineF r sim p1 p2 t1 t2)
-    {p1 p2 : PartENat} {t1 : CTree ε ρ} {t2 : CTree ε σ} (h : sim p1 p2 t1 t2) : t1 ⊑r⊑ t2 :=
+    (p1 p2 : PartENat) {t1 : CTree ε ρ} {t2 : CTree ε σ} (h : sim p1 p2 t1 t2) : t1 ⊑r⊑ t2 :=
     ⟨p1, ⟨p2, Refine'.fixpoint_induct r sim adm p1 p2 t1 t2 h⟩⟩
 
   @[refl]
   theorem Refine.refl {r : Rel ρ ρ} [IsRefl ρ r] (t : CTree ε ρ) : t ⊑r⊑ t := by
-    sorry
+    apply Refine.coind (λ p1 p2 t1 t2 => p1 = 0 ∧ p2 = 0 ∧ t1 = t2) _ 0 0 (And.intro rfl <| And.intro rfl rfl)
+    intro p1 p2 t t' h
+    obtain ⟨hp1, hp2, heq⟩ := h
+    subst hp1
+    subst hp2
+    subst heq
+    apply dMatchOn t
+    · intro v heq
+      subst heq
+      apply RefineF.ret
+      exact IsRefl.refl v
+    · intro c heq
+      subst heq
+      apply RefineF.tau_left
+      apply RefineF.tau_right
+      apply RefineF.coind 0 0
+      <;> simp_all only [PartENat.zero_lt_top]
+      simp_all only [and_self]
+    · intro α e k heq
+      subst heq
+      apply RefineF.vis
+      intro a
+      apply RefineF.coind 0 0
+      <;> simp_all only [PartENat.zero_lt_top]
+      simp_all only [and_self]
+    · intro heq
+      subst heq
+      exact RefineF.zero
+    · intro c1 c2 heq
+      subst heq
+      apply RefineF.choice_idemp
+      · apply RefineF.choice_left
+        apply RefineF.coind 0 0
+        <;> simp_all only [PartENat.zero_lt_top]
+        simp_all only [and_self]
+      · apply RefineF.choice_right
+        apply RefineF.coind 0 0
+        <;> simp_all only [PartENat.zero_lt_top]
+        simp_all only [and_self]
 
   @[trans]
   theorem Refine.trans {r1 : Rel α β} {r2 : Rel β γ} {t1 : CTree ε α} {t2 : CTree ε β} {t3 : CTree ε γ}
